store/client_proofs/close.v
@@ -36,7 +36,7 @@ Lemma wp_client_close c kI kR cs :
 Proof.
 iIntros "#chan_c (_ & _ & _ & _ & _ & _ & _ & _ & #close & #ack & _)".
 iIntros "!> %Φ client post".
-iDestruct "client" as "(%n & %n0 & client & conn & token)".
+iDestruct "client" as "(%n & client & conn & token)".
 iPoseProof (Conn.connected_keyE with "conn") as "[-> ->]".
 wp_lam. wp_pures.
 wp_apply (@wp_nil term).
@@ -47,7 +47,7 @@ wp_apply (Conn.wp_read with "[//] [] [$]") => //.
 iIntros "%ts (conn & _ & #inv)".
 wp_pures.
 iAssert (|={⊤}=>
-  ∃ failed, Conn.client_disconnected N (si_init cs) (si_resp cs) (n + n0) failed)%I
+  ∃ failed, Conn.client_disconnected N (si_init cs) (si_resp cs) n failed)%I
   with "[token]" as ">(%failed & dis)".
 { iDestruct "token" as "(%e_rl & #server & end)".
   iDestruct "inv" as "[fail|inv]".
@@ -55,7 +55,7 @@ iAssert (|={⊤}=>
     by iApply (Conn.session_failed_failure with "fail").
   - iMod (escrowE with "inv end") as ">c1" => //.
     iExists false. iModIntro. iSplit => //. }
-iDestruct "conn" as "(_ & _ & _ & _ & rel & ts & _)".
+iDestruct "conn" as "(% & % & _ & _ & _ & _ & _ & _ & rel & ts & _)".
 wp_apply (Conn.wp_close with "[$]"). iIntros "_".
 iApply "post". by iFrame.
 Qed.
