store/client_proofs/create.v
@@ -41,7 +41,7 @@ Lemma wp_client_create c kI kR cs t1 t2 :
 Proof.
 iIntros "#chan_c (_ & _ & _ & _ & #create & #ack & _) #p_t1 #p_t2".
 iIntros "!> %Φ [client free] post".
-iDestruct "client" as "(%n & %beginning & client & conn & token)".
+iDestruct "client" as "(%n & client & conn & token)".
 iMod (@rem_mapsto_alloc _ _ _ _ _ _ _ t1 t2 with "client free")
   as "(client & mapsto & _ & #created)".
 { by rewrite elem_of_singleton. }
