store/server_proofs/close.v
@@ -29,14 +29,14 @@ Variable N : namespace.
 
 Ltac failure := iLeft; iFrame.
 
-Lemma wp_server_handle_close c skI skR cs n n0 vdb :
+Lemma wp_server_handle_close c skI skR cs n vdb :
   Conn.cs_role cs = Resp →
   channel c -∗
   store_ctx N -∗
   Conn.handler_correct
-    (server_db_connected' N skI skR cs n n0 vdb)
-    (server_handler_post N skI skR cs n0 vdb)
-    skI skR cs n n0
+    (server_db_connected' N skI skR cs n vdb)
+    (server_handler_post N skI skR cs vdb)
+    skI skR cs n
     (N.@"conn".@"close", Server.handle_close N c (repr cs) vdb).
 Proof.
 iIntros "%e_rl #chan_c #ctx".
@@ -45,34 +45,35 @@ iPoseProof (Conn.ctx_close with "ctx") as "?".
 iPoseProof (Conn.ctx_ack_close with "ctx") as "?".
 rewrite /Conn.handler_correct /=. wp_lam; wp_pures. iModIntro.
 iExists _. iSplit => //.
-iIntros "!> %ts conn _ _ db". wp_pures.
+iIntros "!> %ts !> %Φ (conn & db & _ & _) post". wp_pures.
+iApply (wp_wand with "[conn db] post").
 iDestruct "db" as "(%db & #p_db & vdb & #db_at & token)".
 iPoseProof (Conn.connected_keyE with "conn") as "%e".
 iAssert (|={⊤}=>
   (Conn.session_failed cs true ∨
-     □ Conn.ack_close_pred N skI skR cs (n + n0) [TInt 0]) ∗
+     □ Conn.ack_close_pred N skI skR cs n [TInt 0]) ∗
   server_db_disconnected N skI skR vdb)%I
   with "[vdb token]" as ">(#? & server)".
 { case: e => -> ->. iFrame.
   iDestruct "db_at" as "[fail|db_at]".
   { iModIntro. do !iSplit => //=; eauto.
-    iExists (n + n0), true. do !iSplit => //=; eauto.
+    iExists n, true. do !iSplit => //=; eauto.
     iApply (Conn.session_failed_failure cs true with "fail [//]"). }
   iDestruct "token" as "[fail|(%n' & c1 & c2)]".
   { iModIntro. do !iSplit => //=; eauto.
-    iExists (n + n0), true. do !iSplit => //=; eauto.
+    iExists n, true. do !iSplit => //=; eauto.
     iApply (Conn.session_failed_failure cs true with "fail [//]"). }
-  iMod (Conn.clock_update N (n + n0) with "c1 c2") as "[c1 c2]".
-  iAssert (|={⊤}=> Conn.conn_closed N cs (n + n0))%I with "[c2]" as ">#?".
+  iMod (Conn.clock_update N n with "c1 c2") as "[c1 c2]".
+  iAssert (|={⊤}=> Conn.conn_closed N cs n)%I with "[c2]" as ">#?".
   { iApply (escrowI with "c2"). iApply term_token_switch. }
   iModIntro. iSplit; eauto.
-  iExists (n + n0), false. do !iSplit => //; eauto.
+  iExists n, false. do !iSplit => //; eauto.
   by iRight. }
 wp_list.
 wp_apply (Conn.wp_write with "[//] [] [] [] [$]") => //.
 { by rewrite /= public_TInt; eauto. }
 iIntros "conn". wp_pures.
-iDestruct "conn" as "(? & ? & ? & ? & rel & ts & _)".
+iDestruct "conn" as "(% & % & _ & _ & ? & ? & ? & ? & rel & ts & _)".
 wp_apply (Conn.wp_close with "ts"). iIntros "_".
 wp_pures. iModIntro. iRight. iExists _. iSplit => //.
 iRight. by iFrame.
